Add operations to block until all other threads finish. Finish log proof.
We now track the number of running threads with a counter. When a thread is
spawned, this counter is incremented, and we append a command called
"Unregister" to the end of the spawned thread that decrements the counter.  A
command called "Wait" blocks until this counter reaches 1 (meaning all other
threads have called Unregister). Crashing and finishing execution resets this
counter to 1.  A "finish_step" relation has been added to layers but is not yet
run at the end of execution.

Client programs in an abstract layer should not directly call Unregister/Wait.
Rather, when compiling we adjoin a call to "Wait" to the end of the first
thread of the compiled program. This is needed for implementations like the
write ahead log, where correctness requires that all client operations in other
threads finish before launching a new program. (The plan is also to
subsequently let layer implementations have a special 'Close()' proc that would
be called after "Wait"). (In principle clients could be allowed to call 'Wait',
but the current refinement theorem forbids this.)

At the logical level, we now have two assertions called
"Registered" and "AllDone". Launched threads get a "Registered" permission.  We
also have a triple for "Wait" which gives an "AllDone" in the post-condition.
Proofs use a rule that says Registered * AllDone |- False to be able to exploit
the fact that other threads should not be running after a call to Wait.

This is used to complete the write-ahead-log example.

src/CSL/Refinement.v
@@ -17,7 +17,7 @@ Set Nested Proofs Allowed.
 
 Definition procT {OpT} := {T : Type & proc OpT T}.
 Canonical Structure procTC OpT := leibnizC (@procT OpT).
-Canonical Structure StateC OpT (Λ: Layer OpT) := leibnizC (State Λ).
+Canonical Structure StateC OpT (Λ: Layer OpT) := leibnizC (OpState Λ).
 
 Section ghost.
 Context {OpT: Type → Type}.
@@ -57,19 +57,19 @@ Section ghost_spec.
     own cfg_name (◯ ({[ j := Excl (existT _ e : procTC OpT) ]}, ε)).
 
   (* ownership of this does not mean there aren't other threads not in (fst ρ) *)
-  Definition source_cfg ρ : iProp Σ :=
-    own cfg_name (◯ (tpool_to_res (fst ρ), Some (Excl (snd ρ)))).
+  Definition source_cfg (ρ: thread_pool OpT * State Λ) : iProp Σ :=
+    own cfg_name (◯ (tpool_to_res (fst ρ), Some (Excl (snd (snd ρ))))).
 
-  Definition source_state (σ: State Λ) : iProp Σ :=
+  Definition source_state (σ: OpState Λ) : iProp Σ :=
     own cfg_name (◯ (∅ : tpoolUR, Some (Excl σ))).
 
   Definition source_pool_map (tp: gmap nat ({T : Type & proc OpT T})) : iProp Σ :=
     own cfg_name (◯ (Excl <$> tp : gmap nat (exclR (procTC OpT)), ε)).
 
-  Definition source_inv (tp: thread_pool OpT) (σ: State Λ) : iProp Σ :=
-    (∃ tp' σ', own cfg_name (● (tpool_to_res tp', Some (Excl σ'))) ∗
-                   ⌜ bind_star (exec_pool Λ.(sem)) tp σ (Val σ' tp')
-                     ∧ ¬ bind_star (exec_pool Λ.(sem)) tp σ Err ⌝)%I.
+  Definition source_inv (tp: thread_pool OpT) (σ: OpState Λ) : iProp Σ :=
+    (∃ tp' n σ', own cfg_name (● (tpool_to_res tp', Some (Excl σ'))) ∗
+                   ⌜ bind_star (exec_pool Λ.(sem)) tp (1, σ) (Val (n, σ') tp')
+                     ∧ ¬ bind_star (exec_pool Λ.(sem)) tp (1, σ) Err ⌝)%I.
 
   Definition source_ctx ρ : iProp Σ :=
     inv sourceN (source_inv (fst ρ) (snd ρ)).
@@ -229,8 +229,8 @@ Section ghost_step.
     * by left.
   Qed.
 
-  Lemma source_cfg_init `{cfgPreG Σ} tp (σ: State Λ) :
-    ¬ bind_star (exec_pool Λ.(sem)) tp σ Err →
+  Lemma source_cfg_init `{cfgPreG Σ} tp (σ: OpState Λ) :
+    ¬ bind_star (exec_pool Λ.(sem)) tp (1, σ) Err →
     (|={⊤}=> ∃ _ : cfgG Σ, source_ctx (tp, σ) ∗ source_pool_map (tpool_to_map tp) ∗ source_state σ)%I.
   Proof.
     intros Hno_err.
@@ -247,7 +247,7 @@ Section ghost_step.
     set (IN := {| cfg_name := γ |}).
     iExists IN.
     iMod (inv_alloc sourceN ⊤ (source_inv tp σ) with "[Hauth]").
-    { rewrite /source_inv. iNext. iExists tp, σ. iFrame "Hauth".
+    { rewrite /source_inv. iNext. iExists tp, 1, σ. iFrame "Hauth".
       iPureIntro; split; eauto. econstructor. }
     iModIntro. iFrame.
     rewrite pair_split.
@@ -255,7 +255,7 @@ Section ghost_step.
   Qed.
 
   Context `{cfgG Σ}.
-  Context `{Inhabited Λ.(State)}.
+  Context `{Inhabited Λ.(OpState)}.
 
   Lemma source_thread_update {T T'} (e': proc OpT T') tp j (e: proc OpT T)  σ :
     j ⤇ e -∗ own cfg_name (● (tpool_to_res tp, Excl' σ))
@@ -345,13 +345,13 @@ Section ghost_step.
 
   Lemma ghost_step_lifting' {T1 T2} E ρ j K `{LanguageCtx OpT T1 T2 Λ K}
              (e1: proc OpT T1) σ1 σ2 e2 efs:
-    Λ.(sem).(exec_step) e1 σ1 (Val σ2 (e2, efs)) →
+    (∀ n, ∃ n', Λ.(sem).(exec_step) e1 (n, σ1) (Val (n', σ2) (e2, efs))) →
     nclose sourceN ⊆ E →
     source_ctx ρ ∗ j ⤇ K e1 ∗ source_state σ1
       ={E}=∗ j ⤇ K e2 ∗ source_state σ2 ∗ [∗ list] ef ∈ efs, ∃ j', j' ⤇ (projT2 ef).
   Proof.
     iIntros (Hstep ?) "(#Hctx&Hj&Hstate)". rewrite /source_ctx/source_inv.
-    iInv "Hctx" as (tp' σ') ">[Hauth %]" "Hclose".
+    iInv "Hctx" as (tp' n' σ') ">[Hauth %]" "Hclose".
 
     (* Reconcile view based on authoritative element *)
     iDestruct (source_thread_reconcile with "Hj Hauth") as %Heq_thread.
@@ -362,14 +362,15 @@ Section ghost_step.
     iMod (source_thread_update (K e2) with "Hj Hauth") as "[Hj Hauth]".
     iMod (source_threads_fork efs with "Hauth") as "[Hj' Hauth]".
     iMod (source_state_update σ2 with "Hstate Hauth") as "[Hstate Hauth]".
+    destruct (Hstep n') as (n''&?).
 
     (* Restore the invariant *)
     iMod ("Hclose" with "[Hauth]").
-    { iNext. iExists (<[j := (existT T2 (K e2))]>tp' ++ efs), σ2.
+    { iNext. iExists (<[j := (existT T2 (K e2))]>tp' ++ efs), n'', σ2.
       iFrame. intuition. iPureIntro; split; auto.
 
       apply bind_star_expand_r_valid.
-      right. exists tp', σ'; split; auto.
+      right. exists tp', (n', σ'); split; auto.
       apply exec_pool_equiv_alt_val.
       econstructor.
       { symmetry; eapply take_drop_middle; eauto. }
@@ -389,7 +390,7 @@ Section ghost_step.
   (* Curried form is more useful, I think *)
   Lemma ghost_step_lifting {T1 T2} E ρ j K `{LanguageCtx OpT T1 T2 Λ K}
              (e1: proc OpT T1) σ1 σ2 e2 efs:
-    Λ.(sem).(exec_step) e1 σ1 (Val σ2 (e2, efs)) →
+    (∀ n, ∃ n', Λ.(sem).(exec_step) e1 (n, σ1) (Val (n', σ2) (e2, efs))) →
     nclose sourceN ⊆ E →
     j ⤇ K e1 -∗ source_ctx ρ -∗ source_state σ1
       ={E}=∗ j ⤇ K e2 ∗ source_state σ2 ∗ [∗ list] ef ∈ efs, ∃ j', j' ⤇ (projT2 ef).
@@ -397,13 +398,13 @@ Section ghost_step.
 
   Lemma ghost_step_lifting_puredet {T1 T2} E ρ j K `{LanguageCtx OpT T1 T2 Λ K}
              (e1: proc OpT T1) e2 efs:
-    (∀ σ1, Λ.(sem).(exec_step) e1 σ1 (Val σ1 (e2, efs))) →
+    (∀ n σ1, ∃ n', Λ.(sem).(exec_step) e1 (n, σ1) (Val (n', σ1) (e2, efs))) →
     nclose sourceN ⊆ E →
     source_ctx ρ ∗ j ⤇ K e1
       ={E}=∗ j ⤇ K e2 ∗ [∗ list] ef ∈ efs, ∃ j', j' ⤇ (projT2 ef).
   Proof.
     iIntros (Hstep ?) "(#Hctx&Hj)". rewrite /source_ctx/source_inv.
-    iInv "Hctx" as (tp' σ') ">[Hauth %]" "Hclose".
+    iInv "Hctx" as (tp' n' σ') ">[Hauth %]" "Hclose".
 
     (* Reconcile view based on authoritative element *)
     iDestruct (source_thread_reconcile with "Hj Hauth") as %Heq_thread.
@@ -412,14 +413,15 @@ Section ghost_step.
     (* Update authoritative resources to simulate step *)
     iMod (source_thread_update (K e2) with "Hj Hauth") as "[Hj Hauth]".
     iMod (source_threads_fork efs with "Hauth") as "[Hj' Hauth]".
+    destruct (Hstep n' σ') as (n''&?).
 
     (* Restore the invariant *)
     iMod ("Hclose" with "[Hauth]").
-    { iNext. iExists (<[j := (existT T2 (K e2))]>tp' ++ efs), _.
+    { iNext. iExists (<[j := (existT T2 (K e2))]>tp' ++ efs), _, _.
       iFrame. intuition. iPureIntro; split; auto.
 
       apply bind_star_expand_r_valid.
-      right. exists tp', σ'; split; auto.
+      right. exists tp', (n', σ'); split; auto.
       apply exec_pool_equiv_alt_val.
       econstructor.
       { symmetry; eapply take_drop_middle; eauto. }
@@ -438,7 +440,7 @@ Section ghost_step.
 
   Lemma ghost_step_lifting_bind' {T1 T2} E ρ j (K: T1 → proc OpT T2)
              (e1: proc OpT T1) σ1 σ2 e2 efs:
-    Λ.(sem).(exec_step) e1 σ1 (Val σ2 (e2, efs)) →
+    (∀ n, ∃ n', Λ.(sem).(exec_step) e1 (n, σ1) (Val (n', σ2) (e2, efs))) →
     nclose sourceN ⊆ E →
     source_ctx ρ ∗ j ⤇ Bind e1 K ∗ source_state σ1
       ={E}=∗ j ⤇ Bind e2 K ∗ source_state σ2 ∗ [∗ list] ef ∈ efs, ∃ j', j' ⤇ (projT2 ef).
@@ -448,7 +450,7 @@ Section ghost_step.
 
   Lemma ghost_step_lifting_bind {T1 T2} E ρ j (K: T1 → proc OpT T2)
              (e1: proc OpT T1) σ1 σ2 e2 efs:
-    Λ.(sem).(exec_step) e1 σ1 (Val σ2 (e2, efs)) →
+    (∀ n, ∃ n', Λ.(sem).(exec_step) e1 (n, σ1) (Val (n', σ2) (e2, efs))) →
     nclose sourceN ⊆ E →
     j ⤇ Bind e1 K -∗ source_ctx ρ -∗ source_state σ1
       ={E}=∗ j ⤇ Bind e2 K ∗ source_state σ2 ∗ [∗ list] ef ∈ efs, ∃ j', j' ⤇ (projT2 ef).
@@ -460,7 +462,7 @@ Section ghost_step.
     j ⤇ K' (Bind (Ret v) K) -∗ source_ctx ρ ={E}=∗ j ⤇ K' (K v).
   Proof.
     iIntros (?) "Hj Hctx". iMod (ghost_step_lifting_puredet with "[Hj Hctx]") as "($&?)"; eauto.
-    { intros. econstructor. }
+    { intros. eexists. econstructor. }
   Qed.
 
   Lemma ghost_step_loop {T1 T2 T3} E ρ j K `{LanguageCtx OpT T2 T3 Λ K}
@@ -469,9 +471,22 @@ Section ghost_step.
     j ⤇ K (Loop body v) -∗ source_ctx ρ ={E}=∗ j ⤇ K (loop1 body v).
   Proof.
     iIntros (?) "Hj Hctx". iMod (ghost_step_lifting_puredet with "[Hj Hctx]") as "($&?)"; eauto.
-    { intros. econstructor. }
+    { intros. eexists. econstructor. }
   Qed.
 
+  Lemma ghost_step_spawn {T T'} E ρ j K `{LanguageCtx OpT unit T Λ K} (e: proc OpT T'):
+    nclose sourceN ⊆ E →
+    j ⤇ K (Spawn e) -∗ source_ctx ρ
+    ={E}=∗ j ⤇ K (Ret tt) ∗ (∃ j', j' ⤇ (Bind e (λ _, Unregister))).
+  Proof.
+    iIntros (?) "Hj Hctx". iMod (ghost_step_lifting_puredet with "[Hj Hctx]") as "($&H)"; eauto.
+    { intros. exists (S n). econstructor.  exists (S n, σ1); split; econstructor; eauto.
+      econstructor; eauto.
+    }
+    iModIntro. iDestruct "H" as "($&_)".
+  Qed.
+
+  (*
   Lemma ghost_step_spawn {T T'} E ρ j K `{LanguageCtx OpT unit T Λ K} (e: proc OpT T') σ:
     nclose sourceN ⊆ E →
     j ⤇ K (Spawn e) -∗ source_state σ -∗ source_ctx ρ
@@ -486,6 +501,7 @@ Section ghost_step.
     }
     iDestruct "H" as "(?&?&?)". by iFrame.
   Qed.
+   *)
 
 End ghost_step.
 End ghost.
