src/Examples/ExMach/Adequacy.v
@@ -9,10 +9,12 @@ Require Export ExMach.ExMachAPI ExMach.WeakestPre.
 Class exmachPreG Σ := ExMachPreG {
   exm_preG_iris :> invPreG Σ;
   exm_preG_mem :> gen_heapPreG nat nat Σ;
-  exm_preG_disk :> gen_heapPreG nat nat Σ
+  exm_preG_disk :> gen_heapPreG nat nat Σ;
+  exm_preG_treg_inG :> inG Σ (csumR countingR (authR (optionUR (exclR unitC))));
 }.
 
-Definition exmachΣ : gFunctors := #[invΣ; gen_heapΣ nat nat; gen_heapΣ nat nat].
+Definition exmachΣ : gFunctors := #[invΣ; gen_heapΣ nat nat; gen_heapΣ nat nat;
+                                    GFunctor (csumR countingR (authR (optionUR (exclR unitC))))].
 Instance subG_exmachPreG {Σ} : subG exmachΣ Σ → exmachPreG Σ.
 Proof. solve_inG. Qed.
 
