src/Examples/ExMach/RefinementAdequacy.v
@@ -43,10 +43,11 @@ Section refinement.
 
   Lemma refinement_triples:
              forall {H1 H2 T1 T2} j K `{LanguageCtx OpT T1 T2 Λa K} (e: proc OpT T1),
+               wf_client e →
                j ⤇ K e ∗ Registered ∗ (@exec_inv H1 H2) ⊢
                  WP compile e {{ v, j ⤇ K (Ret v) ∗ Registered }}.
   Proof.
-    intros ???? j K Hctx e.
+    intros ???? j K Hctx e Hwf.
     iIntros "(Hj&Hreg&#Hinv)".
     iAssert (⌜∃ ea: Λa.(State), True⌝)%I as %[? _].
     {
@@ -55,20 +56,24 @@ Section refinement.
     }
     assert (Inhabited Λa.(State)).
     { eexists. eauto. }
+    assert (Inhabited Λa.(OpState)).
+    { eexists. destruct x; eauto. }
     iInduction e as [] "IH" forall (j T2 K Hctx).
     - iApply refinement_op_triples; iFrame; eauto.
     - wp_ret. iFrame.
     - wp_bind.
       iApply wp_wand_l. iSplitL ""; last first.
-      * iApply ("IH1" $! _ _ (fun x => K (Bind x p2)) with "[] Hj"); try iFrame.
+      * unshelve (iApply ("IH1" $! _ _ _ (fun x => K (Bind x p2)) with "[] Hj"); try iFrame).
+        { eapply Hwf. }
         { iPureIntro. apply comp_ctx; auto. apply _. }
       * iIntros (?) "(Hj&Hreg)".
         iDestruct (exec_inv_source_ctx with "Hinv") as (?) "#Hctx".
         iMod (ghost_step_bind_ret with "Hj []") as "Hj".
         { set_solver+. }
         { eauto. }
-        iApply ("IH" with "[//] Hj Hreg"); auto.
-    - iLöb as "IHloop" forall (init).
+        iApply ("IH" with "[] [] Hj Hreg"); auto.
+        { iPureIntro. eapply Hwf. }
+    - iLöb as "IHloop" forall (init Hwf).
       iDestruct (exec_inv_source_ctx with "Hinv") as (?) "#Hctx".
       iMod (ghost_step_loop with "Hj []") as "Hj".
       { set_solver+. }
@@ -77,11 +82,12 @@ Section refinement.
       iApply wp_wand_l.
       iSplitL ""; last first.
       * rewrite /loop1. simpl.
-        iApply ("IH" $! _ _ _ (fun x => K (Bind x
+        unshelve (iApply ("IH" $! _ _ _ _ (fun x => K (Bind x
                                (fun out => match out with
                                | ContinueOutcome x => Loop body x
                                | DoneWithOutcome r => Ret r
-                               end))) with "[] Hj Hreg")%proc.
+                               end))) with "[] Hj Hreg")%proc).
+        { eauto. }
         { iPureIntro. apply comp_ctx; auto. apply _. }
       * iIntros (out) "(Hj&Hreg)".
         destruct out.
@@ -89,37 +95,46 @@ Section refinement.
            iMod (ghost_step_bind_ret with "Hj []") as "Hj".
            { set_solver+. }
            { eauto. }
-           iApply ("IHloop" with "Hj Hreg").
+           iApply ("IHloop" with "[] Hj Hreg").
+           { eauto. }
         ** iNext.
            iMod (ghost_step_bind_ret with "Hj []") as "Hj".
            { set_solver+. }
            { eauto. }
            wp_ret. iFrame.
-   - simpl. iApply (wp_unregister with "Hreg"). iNext  refinement_op_triples; iFrame; eauto.
+   - inversion Hwf.
+   - inversion Hwf.
    - iDestruct (exec_inv_source_ctx with "Hinv") as (?) "#Hctx".
      iMod (ghost_step_spawn with "Hj []") as "(Hj&Hj')".
      { set_solver+. }
      { eauto. }
      iDestruct "Hj'" as (j') "Hj'".
-     iApply (wp_spawn with "[Hj'] [Hj]").
-     { iNext. iApply wp_wand_l; iSplitL ""; last first.
-       { iApply ("IH" $! _ _ (fun x => x)); first (iPureIntro; apply _).
-         iFrame. }
-       eauto. }
-     eauto.
+     iApply (wp_spawn with "Hreg [Hj'] [Hj]").
+     { iNext. iIntros "Hreg'". 
+       { wp_bind.
+         iApply (wp_wand with "[Hj' Hreg'] []").
+         { unshelve (iApply ("IH" $! _ _ _ (fun x => Bind x (fun _ => Unregister))
+                               with "[] Hj' Hreg'")).
+           { eauto. }
+           { iPureIntro. apply _. }
+         }
+         { iIntros (?) "(?&?)". iApply (wp_unregister with "[$]"). iIntros "!> ?". eauto. }
+       }
+     }
+     iIntros "!> ?". iFrame.
   Qed.
 
   Context (recv_triple:
              forall {H1 H2} param,
-               (@crash_inv H1 H2 param) ∗ (@crash_starter H1 H2 param) ⊢
+               (@crash_inv H1 H2 param) ∗ Registered ∗ (@crash_starter H1 H2 param) ⊢
                     WP recv @ NotStuck; ⊤ {{ v, |={⊤,E}=> ∃ σ2a σ2a', source_state σ2a
                     ∗ ⌜Λa.(crash_step) σ2a (Val σ2a' tt)⌝ ∗
-                    ∀ `{Hcfg': cfgG OpT Λa Σ} (Hinv': invG Σ) ρ,
+                    ∀ `{Hcfg': cfgG OpT Λa Σ} (Hinv': invG Σ) tr' ρ,
                       source_ctx (ρ, σ2a') ∗ source_state σ2a'  ={⊤}=∗
-                      exec_inner Hcfg' (ExMachG Σ Hinv' exm_mem_inG exm_disk_inG)
+                      exec_inner Hcfg' (ExMachG Σ Hinv' exm_mem_inG exm_disk_inG tr')
                                                }}).
 
-  Context (init_absr: Λa.(State) → ExMach.State → Prop).
+  Context (init_absr: Λa.(OpState) → ExMach.State → Prop).
   Context (init_wf: ∀ σ1a σ1c, init_absr σ1a σ1c → state_wf σ1c).
 
   Context (init_exec_inner: ∀ σ1a σ1c ρ, init_absr σ1a σ1c →
@@ -130,84 +145,93 @@ Section refinement.
 
   Context (exec_inv_preserve_crash:
       (∀ `{Hex: exmachG Σ} `{Hcfg: cfgG OpT Λa Σ},
-          exec_inv Hcfg Hex ={⊤, E}=∗ ∀ Hmem',
-          (let Hex := ExMachG Σ (exm_invG) Hmem' (exm_disk_inG) in
+          exec_inv Hcfg Hex ={⊤, E}=∗ ∀ Hmem' Hreg',
+          (let Hex := ExMachG Σ (exm_invG) Hmem' (exm_disk_inG) Hreg' in
               ([∗ map] i ↦ v ∈ init_zero, i m↦ v) ={E}=∗ crash_inner Hcfg Hex))).
 
   Context (crash_inv_preserve_crash:
       (∀ `{Hex: exmachG Σ} `{Hcfg: cfgG OpT Λa Σ} param,
-          crash_inv Hcfg Hex param ={⊤, E}=∗ ∀ Hmem',
-          (let Hex := ExMachG Σ (exm_invG) Hmem' (exm_disk_inG) in
+          crash_inv Hcfg Hex param ={⊤, E}=∗ ∀ Hmem' Hreg',
+          (let Hex := ExMachG Σ (exm_invG) Hmem' (exm_disk_inG) Hreg' in
               ([∗ map] i ↦ v ∈ init_zero, i m↦ v) ={E}=∗ crash_inner Hcfg Hex))).
 
   (* TODO: Much of this business is just to capture the fact that exec_inner/crash_inner
      should not really mention invariants, because those old invariants are 'dead' *)
   Context (crash_inner_inv :
       (∀ `{Hex: exmachG Σ} `{Hcfg: cfgG OpT Λa Σ} cfg,
-          (∃ Hinv, crash_inner Hcfg (ExMachG Σ Hinv (exm_mem_inG) (exm_disk_inG))) ∗
+          (∃ Hinv, crash_inner Hcfg (ExMachG Σ Hinv (exm_mem_inG) (exm_disk_inG) (exm_treg_inG))) ∗
           source_ctx cfg
           ={⊤}=∗ ∃ param, crash_inv Hcfg Hex param ∗ crash_starter Hcfg Hex param)).
 
   Context (exec_inner_inv :
       (∀ `{Hex: exmachG Σ} `{Hcfg: cfgG OpT Λa Σ} cfg,
-          (∃ Hinv, exec_inner Hcfg (ExMachG Σ Hinv (exm_mem_inG) (exm_disk_inG))) ∗
+          (∃ Hinv, exec_inner Hcfg (ExMachG Σ Hinv (exm_mem_inG) (exm_disk_inG) (exm_treg_inG))) ∗
           source_ctx cfg
           ={⊤}=∗ exec_inv Hcfg Hex)).
 
   Context (inv_implies_source:
              ∀ `{Hex: exmachG Σ} `{Hcfg: cfgG OpT Λa Σ},
-             exec_inv Hcfg Hex ={⊤, E}=∗ ∃ σ2a : Λa.(State), source_state σ2a).
+             AllDone -∗ exec_inv Hcfg Hex ={⊤, E}=∗ ∃ σ2a : Λa.(OpState), source_state σ2a).
 
   (* TODO: should we model explicit effects of finishing programs? *)
   Context (exec_inv_preserve_finish:
       (∀ `{Hex: exmachG Σ} `{Hcfg: cfgG OpT Λa Σ},
-          exec_inv Hcfg Hex ={⊤, E}=∗ ∃ σ2a : Λa.(State), source_state σ2a ∗
-          ∀ `{Hcfg': cfgG OpT Λa Σ} (Hinv': invG Σ) ρ,
+          AllDone -∗ exec_inv Hcfg Hex ={⊤, E}=∗ ∃ σ2a : Λa.(OpState), source_state σ2a ∗
+          ∀ `{Hcfg': cfgG OpT Λa Σ} (Hinv': invG Σ) Hreg' ρ,
             source_ctx (ρ, σ2a) ∗ source_state σ2a  ={⊤}=∗
-             exec_inner Hcfg' (ExMachG Σ Hinv' exm_mem_inG exm_disk_inG))).
+             exec_inner Hcfg' (ExMachG Σ Hinv' exm_mem_inG exm_disk_inG Hreg'))).
 
 
   Lemma exmach_crash_refinement_seq {T} σ1c σ1a (es: proc_seq OpT T) :
     init_absr σ1a σ1c →
-    ¬ proc_exec_seq Λa es (rec_singleton (Ret ())) σ1a Err →
-    ∀ σ2c res, ExMach.l.(proc_exec_seq) (compile_proc_seq es) (rec_singleton recv) σ1c (Val σ2c res) →
-    ∃ σ2a, Λa.(proc_exec_seq) es (rec_singleton (Ret tt)) σ1a (Val σ2a res).
+    wf_client_seq es →
+    ¬ proc_exec_seq Λa es (rec_singleton (Ret ())) (1, σ1a) Err →
+    ∀ σ2c res, ExMach.l.(proc_exec_seq) (compile_proc_seq es)
+                                        (rec_singleton recv) (1, σ1c) (Val σ2c res) →
+    ∃ σ2a, Λa.(proc_exec_seq) es (rec_singleton (Ret tt)) (1, σ1a) (Val σ2a res).
   Proof.
-    rewrite /compile_proc_seq. intros Hinit Hno_err.
+    rewrite /compile_proc_seq. intros Hinit Hwf_seq Hno_err.
     unshelve (eapply wp_proc_seq_refinement_adequacy with
                   (φ := fun _ _ _ => True%I)
                   (φrec := fun _ _ => True%I)
                   (E0 := E); eauto).
     clear Hno_err.
   iAssert (∀ invG H1 ρ, |={⊤}=>
-       ∃ hM hD
+       ∃ hM hD tR
             (Hmpf_eq : hM.(@gen_heap_inG addr nat Σ nat_eq_dec nat_countable) =
           H.(@exm_preG_disk Σ).(@gen_heap_preG_inG addr nat Σ nat_eq_dec nat_countable))
             (Hdpf_eq : hD.(@gen_heap_inG addr nat Σ nat_eq_dec nat_countable) =
           H.(@exm_preG_disk Σ).(@gen_heap_preG_inG addr nat Σ nat_eq_dec nat_countable)),
-         (@ex_mach_interp _ hM hD σ1c) ∗
+         (@ex_mach_interp _ hM hD {| treg_name := tR; treg_counter_inG := _ |} (1, σ1c)) ∗
          (source_ctx (ρ, σ1a) -∗ source_state σ1a ={⊤}=∗
-       exec_inner H1 (ExMachG Σ invG hM hD)))%I as "Hpre".
+         own tR (Cinl (Count (-1))) ∗ 
+          exec_inner H1 (ExMachG Σ invG hM hD {| treg_name := tR; treg_counter_inG := _ |})))%I
+      as "Hpre".
   {
   iIntros.
   iMod (gen_heap_strong_init (mem_state σ1c)) as (hM Hmpf_eq) "(Hmc&Hm)".
   iMod (gen_heap_strong_init (disk_state σ1c)) as (hD Hdpf_eq) "(Hdc&Hd)".
-  iModIntro. iExists hM, hD, Hmpf_eq, Hdpf_eq. iSplitL "Hmc Hdc".
-  { iExists _, _. iFrame. iPureIntro.
+  iMod (own_alloc (Cinl (Count 0))) as (tR) "Ht".
+  { constructor. }
+  set (tR' := {| treg_name := tR; treg_counter_inG := _ |}).
+  iAssert (own tR (Cinl (Count 1)) ∗ own tR (Cinl (Count (-1))))%I with "[Ht]" as "(Ht&Hreg)".
+  { rewrite /Registered -own_op Cinl_op counting_op' //=. }
+  iModIntro. iExists hM, hD, tR, Hmpf_eq, Hdpf_eq. iSplitL "Hmc Hdc Ht".
+  { iFrame. iExists _, _. iFrame. iPureIntro.
     edestruct (init_wf) as (Hwf1&Hwf2); eauto.
     split_and!; eauto; intros i.
     * destruct (Hwf1 i); intuition.
     * destruct (Hwf2 i); intuition.
   }
   iIntros.
-  iPoseProof (init_exec_inner σ1a σ1c ρ Hinit (ExMachG Σ _ hM hD) _) as "H".
-  iMod ("H" with "[-]") as "$".
+  iPoseProof (init_exec_inner σ1a σ1c ρ Hinit (ExMachG Σ _ hM hD tR') _) as "H".
+  iMod ("H" with "[-Hreg]") as "$".
   { iFrame.  iSplitL "Hm"; [| iSplitL "Hd"].
     { rewrite -Hmpf_eq. iApply mem_init_to_bigOp; auto. }
     { rewrite -Hdpf_eq. iApply disk_init_to_bigOp; auto. }
     eauto.
   }
-  eauto.
+  iFrame; eauto.
   }
 
   clear Hinit.
@@ -215,59 +239,83 @@ Section refinement.
   - iSplit; first by eauto.
   iExists (fun cfgG s => ∃ (_ : exmachG Σ),
                      state_interp s ∗
-                       (∃ (hM: gen_heapG addr nat Σ)
+                       (∃ (hM: gen_heapG addr nat Σ) tr
                             (Hmpf_eq : hM.(@gen_heap_inG addr nat Σ nat_eq_dec nat_countable) =
                                        H.(@exm_preG_disk Σ).(@gen_heap_preG_inG addr nat Σ
                                                               nat_eq_dec nat_countable)) ,
-            gen_heap_ctx init_zero ∗ crash_inner cfgG (ExMachG Σ _ hM (exm_disk_inG))))%I; auto.
+            gen_heap_ctx init_zero ∗ own tr (Cinl (Count 0)) ∗ crash_inner cfgG (ExMachG Σ _ hM (exm_disk_inG) {| treg_name := tr; treg_counter_inG := _ |})))%I; auto.
   iIntros (invG0 Hcfg0).
-  iMod ("Hpre" $! invG0 _ _) as (hM hD ??) "(Hstate0&H)".
-  iExists (@ex_mach_interp _ hM hD).
+  iMod ("Hpre" $! invG0 _ _) as (hM hD tR ??) "(Hstate0&H)".
+  set (tR' := {| treg_name := tR; treg_counter_inG := _ |}).
+  iExists (@ex_mach_interp _ hM hD tR').
   iIntros "!> (#Hsrc&Hpt0&Hstate)".
-  iMod ("H" with "Hsrc Hstate") as "Hinv".
-  iMod (exec_inner_inv (ExMachG Σ _ hM hD) _ with "[Hinv]") as "#Hinv".
+  iMod ("H" with "Hsrc Hstate") as "(Hreg&Hinv)".
+  iMod (exec_inner_inv (ExMachG Σ _ hM hD tR') _ with "[Hinv]") as "#Hinv".
   { iFrame. iFrame "Hsrc". iExists _. iFrame. }
   simpl.
   iModIntro.
   iFrame "Hstate0".
-  iSplitL "Hpt0".
-  {  iPoseProof (@wp_mono with "[Hpt0]") as "H"; swap 1 2.
-     { iApply refinement_triples. iFrame. iFrame "Hinv". }
+  iSplitL "Hpt0 Hreg".
+  {  iPoseProof (@wp_mono with "[Hpt0 Hreg]") as "H"; swap 1 2.
+     { iApply refinement_triples. eauto. iFrame "Hinv". iFrame. }
      { reflexivity. }
+     simpl. rewrite /compile_whole.
+     wp_bind.
      iApply (wp_wand with "H [Hinv]").
-     iIntros (v) "Hpt0". iFrame.
-     iIntros (σ2c) "Hmach".
-     iMod (inv_implies_source with "Hinv") as (σ2a) "H".
+     iIntros (v) "(Hpt0&Hreg)".
+     wp_bind.
+     iApply (@wp_wait Σ {| exm_invG := invG0;
+             exm_mem_inG := hM;
+             exm_disk_inG := hD;
+             exm_treg_inG := {| treg_counter_inG := H.(@exm_preG_treg_inG Σ); treg_name := tR |} |}
+               with "Hreg").
+     iIntros "!> Hdone".
+     wp_ret. iFrame. iIntros.
+     iMod (inv_implies_source with "Hdone Hinv") as (σ2a) "H".
      iModIntro. iExists _; iFrame; auto.
   }
   iSplit.
   { iIntros (σ2c) "Hmach".
     iMod (exec_inv_preserve_crash with "Hinv") as "Hinv_post".
     iMod (gen_heap_strong_init (init_zero)) as (hM' Hmpf_eq') "(Hmc&Hm)".
-    iMod ("Hinv_post" with "[Hm]") as "Hinv'".
+    iMod (own_alloc (Cinl (Count 0))) as (tR_fresh) "Ht".
+    { constructor. }
+    set (tR'' := {| treg_name := tR_fresh; treg_counter_inG := _ |}).
+    iMod ("Hinv_post" $! _ tR'' with "[Hm]") as "Hinv'".
     { rewrite -Hmpf_eq'. iApply @mem_init_to_bigOp; auto. }
     iIntros. iModIntro.
-    iExists (ExMachG Σ _ hM hD). iFrame "Hmach".
-    iExists hM', Hmpf_eq'. iFrame.
+    iExists (ExMachG Σ _ hM hD tR'). iFrame "Hmach".
+    iExists hM', tR_fresh, Hmpf_eq'. iFrame.
   }
 
   iClear "Hsrc".
   iModIntro. iIntros (invG Hcfg' ?? Hcrash) "(Hinv0&#Hsrc)".
   iDestruct "Hinv0" as (HexmachG') "(Hinterp&Hinv0)".
-  iDestruct "Hinv0" as (hM' Hmpf_eq') "(Hmc'&Hcrash_inner)".
+  iDestruct "Hinv0" as (hM' tR_fresh Hmpf_eq') "(Hmc'&Hreg&Hcrash_inner)".
   iClear "Hinv".
-  iMod (crash_inner_inv (ExMachG Σ invG hM' (exm_disk_inG)) Hcfg' with "[Hcrash_inner]") as
+  set (tR'' := {| treg_name := tR_fresh; treg_counter_inG := _ |}).
+  iMod (crash_inner_inv (ExMachG Σ invG hM' (exm_disk_inG) tR'') Hcfg' with "[Hcrash_inner]") as
       (param) "(#Hinv&Hstarter)".
-  { iIntros. simpl. iFrame "Hsrc". iExists ( exmachG_irisG.(@iris_invG Op ExMach.State Σ)).
+  { iIntros. simpl. iFrame "Hsrc". iExists ( exmachG_irisG.(@iris_invG Op _ Σ)).
     iFrame. }
   iModIntro.
-  iExists (@ex_mach_interp Σ hM' (exm_disk_inG)).
-  iSplitL "Hinterp Hmc'".
+  iAssert (own tR_fresh (Cinl (Count 1)) ∗ own tR_fresh (Cinl (Count (-1))))%I
+    with "[Hreg]" as "(Ht&Hreg)".
+  { rewrite /Registered -own_op Cinl_op counting_op' //=. }
+  iExists (@ex_mach_interp Σ hM' (exm_disk_inG) tR'').
+  iSplitL "Hinterp Ht Hmc'".
   { (* shows ex_mach_interp is holds after crash for next gen *)
+    rewrite /ex_mach_interp'.
     rewrite /ex_mach_interp.
+    destruct a, a0.
+    iDestruct "Hinterp" as "(?&Hinterp)".
     iDestruct "Hinterp" as (mems disks) "(Hdisks&?&%&Hp)".
     iDestruct "Hp" as %(Hdisks&Hwf1'&Hwf2').
-    inversion Hcrash; subst.
+    destruct Hcrash as ([]&(?&?)&Hput&Hrest).
+    inversion Hput. inversion H4. subst.
+    inversion Hrest; subst. inversion H3. subst.
+    iSplitL "Ht".
+    { iFrame. }
     iExists init_zero, _.
     iFrame.
     iPureIntro. split_and!.
@@ -279,34 +327,42 @@ Section refinement.
       apply is_Some_None in Hsome; auto.
     * rewrite /crash_fun; auto.
   }
-  iSplitL "Hinv Hstarter".
+  iSplitL "Hinv Hreg Hstarter".
   {
-    iPoseProof (@wp_mono with "[Hinv Hstarter]") as "H"; swap 1 2.
+    iPoseProof (@wp_mono with "[Hinv Hreg Hstarter]") as "H"; swap 1 2.
     { iApply recv_triple. iFrame. iApply "Hinv". }
     { reflexivity. }
     iApply (@wp_mono with "H").
     iIntros (_) "H". iIntros (σ2c) "Hinterp".
     iMod "H". iModIntro.
     iDestruct "H" as (σ2a σ2a') "(Hsource&Hinner&Hp)".
-    iExists _, _. iFrame.
+    iExists (1, σ2a), (1, σ2a'). iFrame "Hsource".
+    rewrite right_id. iDestruct "Hinner" as %?. iPureIntro.
+    { eexists tt, (1, σ2a). split; eauto. split; eauto. econstructor; eauto. econstructor; eauto.
+      }
   }
   {
     iIntros (σ2c) "Hmach".
     iMod (crash_inv_preserve_crash with "Hinv") as "Hinv_post".
     iMod (gen_heap_strong_init (init_zero)) as (hM'' Hmpf_eq'') "(Hmc&Hm)".
+    iMod (own_alloc (Cinl (Count 0))) as (tR_fresh') "Ht".
+    { constructor. }
+    set (tR''' := {| treg_name := tR_fresh'; treg_counter_inG := _ |}).
+    iIntros. 
     iMod ("Hinv_post" with "[Hm]") as "Hinv'".
     { rewrite -Hmpf_eq''. iApply @mem_init_to_bigOp; auto. }
-    iIntros. iModIntro.
-
+    iModIntro.
     iExists {| exm_invG := invG;
                exm_mem_inG := hM';
-               exm_disk_inG := HexmachG'.(@exm_disk_inG Σ) |}.
-    iFrame. iExists hM'', Hmpf_eq''. iFrame.
+               exm_disk_inG := HexmachG'.(@exm_disk_inG Σ);
+               exm_treg_inG := tR''
+            |}.
+    iFrame. iExists hM'', tR_fresh', Hmpf_eq''. iFrame.
   }
   -
     iSplit; first by eauto.
   iExists (fun cfgG s => ∃ (Hex : exmachG Σ), state_interp s ∗
-            (∃ (hM: gen_heapG addr nat Σ)
+            (∃ (hM: gen_heapG addr nat Σ) tr
                (Hmpf_eq : hM.(@gen_heap_inG addr nat Σ nat_eq_dec nat_countable) =
                           H.(@exm_preG_disk Σ).(@gen_heap_preG_inG addr nat Σ
                                                                    nat_eq_dec nat_countable))
@@ -314,31 +370,52 @@ Section refinement.
                                                                nat_eq_dec nat_countable)=
                           H.(@exm_preG_disk Σ).(@gen_heap_preG_inG addr nat Σ
                                                                    nat_eq_dec nat_countable)) ,
-            gen_heap_ctx init_zero ∗ crash_inner cfgG (ExMachG Σ _ hM (exm_disk_inG))))%I; auto.
+            gen_heap_ctx init_zero ∗ own tr (Cinl (Count 0)) ∗ crash_inner cfgG (ExMachG Σ _ hM (exm_disk_inG) {| treg_name := tr; treg_counter_inG := _ |})))%I; auto.
   iIntros (invG0 Hcfg0).
-  iMod ("Hpre" $! invG0 _ _) as (hM hD ??) "(Hstate0&H)".
-  iExists (@ex_mach_interp _ hM hD).
+  iMod ("Hpre" $! invG0 _ _) as (hM hD tr ??) "(Hstate0&H)".
+  set (tR' := {| treg_name := tr; treg_counter_inG := _ |}).
+  iExists (@ex_mach_interp _ hM hD tR').
   iIntros "!> (#Hsrc&Hpt0&Hstate)".
-  iMod ("H" with "Hsrc Hstate") as "Hinv".
-  iMod (exec_inner_inv (ExMachG Σ _ hM hD) _ with "[Hinv]") as "#Hinv".
+  iMod ("H" with "Hsrc Hstate") as "(Hreg&Hinv)".
+  iMod (exec_inner_inv (ExMachG Σ _ hM hD tR') _ with "[Hinv]") as "#Hinv".
   { iFrame "Hsrc".  iFrame. iExists _. iFrame. }
   simpl.
   iModIntro.
   iFrame "Hstate0".
-  iSplitL "Hpt0".
-  {  iPoseProof (@wp_mono with "[Hpt0]") as "H"; swap 1 2.
-     { iApply refinement_triples. iFrame. iFrame "Hinv". }
+  iSplitL "Hpt0 Hreg".
+  {  iPoseProof (@wp_mono with "[Hpt0 Hreg]") as "H"; swap 1 2.
+     { iApply refinement_triples. destruct (Hwf_seq) as (?&?). eauto. iFrame. iFrame "Hinv".
+       iFrame "Hreg".
+     }
      { reflexivity. }
+     simpl. rewrite /compile_whole.
+     wp_bind.
      iApply (wp_wand with "H [Hinv]").
-     iIntros (v) "Hpt0". iFrame.
-     iIntros (σ2c) "Hmach".
-     iMod (exec_inv_preserve_finish with "Hinv") as (σ2a) "(H&Hfinish)".
+     iIntros (v) "(Hpt0&Hreg)". iFrame.
+     wp_bind.
+     iApply (@wp_wait Σ {| exm_invG := invG0;
+             exm_mem_inG := hM;
+             exm_disk_inG := hD;
+             exm_treg_inG := tR' |}
+               with "Hreg").
+     iIntros "!> Hdone".
+     wp_ret. iFrame. iIntros (σ2c) "Hmach".
+     iMod (exec_inv_preserve_finish with "Hdone Hinv") as (σ2a) "(H&Hfinish)".
      iModIntro. iExists _; iFrame; auto.
      simpl.
      rewrite -/wp_proc_seq_refinement.
      iApply "IH".
-     { iIntros. iModIntro.
-       iExists hM. iExists hD. unshelve (iExists _, _); try eauto.
+     { iPureIntro. destruct Hwf_seq. eauto. }
+     { iIntros.
+       iMod (own_alloc (Cinl (Count 0))) as (tR_fresh') "Ht".
+       { constructor. }
+       iAssert (own tR_fresh' (Cinl (Count 1))
+                    ∗ own tR_fresh' (Cinl (Count (-1))))%I with "[Ht]" as "(Ht&Hreg)".
+       { rewrite /Registered -own_op Cinl_op counting_op' //=. }
+       set (tR''' := {| treg_name := tR_fresh'; treg_counter_inG := _ |}).
+       iModIntro.
+       iExists hM. iExists hD. iExists tR_fresh'. unshelve (iExists _, _); try eauto.
+       destruct σ2c. iDestruct "Hmach" as "(?&?)".
        iFrame. iIntros. iMod ("Hfinish" with "[-]"). iFrame. eauto.
        iModIntro. eauto.
      }
@@ -347,30 +424,44 @@ Section refinement.
   { iIntros (σ2c) "Hmach".
     iMod (exec_inv_preserve_crash with "Hinv") as "Hinv_post".
     iMod (gen_heap_strong_init (init_zero)) as (hM' Hmpf_eq') "(Hmc&Hm)".
+    iMod (own_alloc (Cinl (Count 0))) as (tR_fresh') "Ht".
+    { constructor. }
+    set (tR''' := {| treg_name := tR_fresh'; treg_counter_inG := _ |}).
     iMod ("Hinv_post" with "[Hm]") as "Hinv'".
     { rewrite -Hmpf_eq'. iApply @mem_init_to_bigOp; auto. }
     iIntros. iModIntro.
-    iExists (ExMachG Σ _ hM hD). iFrame "Hmach".
-    iExists hM', Hmpf_eq', H2. iFrame.
+    iExists (ExMachG Σ _ hM hD tR'). iFrame "Hmach".
+    iExists hM', tR_fresh', Hmpf_eq', H2. iFrame.
   }
   iClear "Hsrc".
   iModIntro. iIntros (invG Hcfg' ?? Hcrash) "(Hinv0&#Hsrc)".
   iDestruct "Hinv0" as (HexmachG') "(Hinterp&Hinv0)".
-  iDestruct "Hinv0" as (hM' Hmpf_eq' Hmdpf_eq') "(Hmc'&Hcrash_inner)".
+  iDestruct "Hinv0" as (hM' tR_fresh' Hmpf_eq' Hmdpf_eq') "(Hmc'&Hreg&Hcrash_inner)".
   iClear "Hinv".
+  set (tR''' := {| treg_name := tR_fresh'; treg_counter_inG := _ |}).
   iMod (crash_inner_inv (ExMachG Σ _
-                                 hM' (exm_disk_inG)) Hcfg'
+                                 hM' (exm_disk_inG) tR''') Hcfg'
                          with "[Hcrash_inner]") as (param) "(#Hinv&Hstarter)".
-  { iIntros. simpl. iFrame "Hsrc". iExists ( exmachG_irisG.(@iris_invG Op ExMach.State Σ)).
+  { iIntros. simpl. iFrame "Hsrc". iExists ( exmachG_irisG.(@iris_invG Op _ Σ)).
     iFrame. }
   iModIntro.
-  iExists (@ex_mach_interp Σ hM' (exm_disk_inG)).
-  iSplitL "Hinterp Hmc'".
+  iAssert (own tR_fresh' (Cinl (Count 1)) ∗ own tR_fresh' (Cinl (Count (-1))))%I
+    with "[Hreg]" as "(Ht&Hreg)".
+  { rewrite /Registered -own_op Cinl_op counting_op' //=. }
+  iExists (@ex_mach_interp Σ hM' (exm_disk_inG) tR''').
+  iSplitL "Hinterp Ht Hmc'".
   { (* shows ex_mach_interp is holds after crash for next gen *)
+    rewrite /ex_mach_interp'.
     rewrite /ex_mach_interp.
+    destruct a, a0.
+    iDestruct "Hinterp" as "(?&Hinterp)".
     iDestruct "Hinterp" as (mems disks) "(Hdisks&?&%&Hp)".
-    iDestruct "Hp" as %(Hdisks&Hwf1&Hwf2).
-    inversion Hcrash; subst.
+    iDestruct "Hp" as %(Hdisks&Hwf1'&Hwf2').
+    destruct Hcrash as ([]&(?&?)&Hput&Hrest).
+    inversion Hput. inversion H4. subst.
+    inversion Hrest; subst. inversion H3. subst.
+    iSplitL "Ht".
+    { iFrame. }
     iExists init_zero, _.
     iFrame.
     iPureIntro. split_and!.
@@ -382,38 +473,56 @@ Section refinement.
       apply is_Some_None in Hsome; auto.
     * rewrite /crash_fun; auto.
   }
-  iSplitL "Hinv Hstarter".
+  iSplitL "Hinv Hreg Hstarter".
   {
-    iPoseProof (@wp_mono with "[Hinv Hstarter IH]") as "H"; swap 1 2.
-    { iApply recv_triple. iFrame "Hstarter". iApply "Hinv". }
+    iPoseProof (@wp_mono with "[Hinv Hreg Hstarter IH]") as "H"; swap 1 2.
+    { iApply recv_triple. iFrame "Hstarter". iFrame. iApply "Hinv". }
     { reflexivity. }
     iApply (@wp_wand with "H [IH]").
     iIntros (_) "H". iIntros (σ2c) "Hinterp".
     iMod "H". iModIntro.
     iDestruct "H" as (σ2a σ2a') "(Hsource&Hinner&Hfinish)".
-    iExists _, _. iFrame.
+    iExists (1, σ2a), (1, σ2a'). iFrame.
      rewrite -/wp_proc_seq_refinement.
+     iDestruct "Hinner" as %?.
+     iSplitL "".
+     { iPureIntro. exists tt, (1, σ2a); split; eauto. econstructor. split; eauto. eauto.
+       econstructor; eauto.
+     }
      iApply "IH".
-     { iIntros. iModIntro.
-       iExists hM'. iExists (HexmachG'.(@exm_disk_inG Σ)). unshelve (iExists _; iExists _); eauto.
-       iFrame "Hinterp".
-       iIntros.
-       iMod ("Hfinish" with "[-]"). iFrame. eauto.
-       iModIntro. eauto.
+     { destruct Hwf_seq. eauto. }
+     { iIntros.
+       iMod (own_alloc (Cinl (Count 0))) as (tR_fresh'') "Ht".
+       { constructor. }
+       iAssert (own tR_fresh'' (Cinl (Count 1))
+                    ∗ own tR_fresh'' (Cinl (Count (-1))))%I with "[Ht]" as "(Ht&Hreg)".
+       { rewrite /Registered -own_op Cinl_op counting_op' //=. }
+       set (tR'''' := {| treg_name := tR_fresh''; treg_counter_inG := _ |}).
+       iModIntro.
+       iExists hM'. iExists (HexmachG'.(@exm_disk_inG Σ)). iExists tR_fresh''.
+       unshelve (iExists _; iExists _); eauto.
+       destruct σ2c. iDestruct "Hinterp" as "(?&?)".
+       iFrame. iIntros. iMod ("Hfinish" with "[-]"). iFrame. eauto.
+       iModIntro. iFrame.
      }
   }
   {
     iIntros (σ2c) "Hmach".
     iMod (crash_inv_preserve_crash with "Hinv") as "Hinv_post".
     iMod (gen_heap_strong_init (init_zero)) as (hM'' Hmpf_eq'') "(Hmc&Hm)".
+    iMod (own_alloc (Cinl (Count 0))) as (tR_fresh'') "Ht".
+    { constructor. }
+    set (tR'''' := {| treg_name := tR_fresh''; treg_counter_inG := _ |}).
     iMod ("Hinv_post" with "[Hm]") as "Hinv'".
     { rewrite -Hmpf_eq''. iApply @mem_init_to_bigOp; auto. }
     iIntros. iModIntro.
 
     iExists {| exm_invG := invG;
                exm_mem_inG := hM';
-               exm_disk_inG := HexmachG'.(@exm_disk_inG Σ) |}.
-    iFrame. unshelve (iExists hM'', Hmpf_eq'', _); eauto. iFrame.
+               exm_disk_inG := HexmachG'.(@exm_disk_inG Σ);
+               exm_treg_inG := tR''' |}.
+    iFrame "Hmach".
+    iFrame. unshelve (iExists hM'', tR_fresh'', Hmpf_eq'', _); eauto. iFrame.
   }
   Qed.
 
